consistency updates, updated push, related is_full refactor and updates

theories/iris/examples/stack/function/is_full.v
@@ -38,9 +38,8 @@ Section code.
   Parameters/Locals:
   0 (input)     stack pointer
 *)
-Definition is_full :=
-  validate_stack 0 ++
-  validate_stack_bound 0 ++
+                 
+Definition is_full_op := 
   [
     i32const 1 ;
     i32const 0 ;
@@ -53,38 +52,24 @@ Definition is_full :=
     BI_select
   ].
 
+Definition is_full :=
+  validate_stack 0 ++ validate_stack_bound 0 ++ is_full_op.
 
 End code.
 
 Section specs.
 
-Lemma spec_is_full f0 n (v : Z) (s : seq.seq i32) E: 
+Lemma spec_is_full_op f0 n (v : Z) (s : seq.seq i32) E: 
   ⊢ {{{ ⌜ f0.(f_inst).(inst_memory) !! 0 = Some n ⌝ ∗
         ⌜ (f_locs f0) !! 0 = Some (value_of_int v) ⌝ ∗ 
         ↪[frame] f0 ∗
         isStack v s n }}}
-    to_e_list is_full @ E
+    to_e_list is_full_op @ E
     {{{ w, ∃ k, ⌜ w = immV [value_of_int k] ⌝ ∗ isStack v s n ∗
-                           ⌜ k = 1 \/ (length s < two14 - 1)%Z ⌝ ∗
-          ∃ f1, ↪[frame] f1 ∗ ⌜ f_inst f0 = f_inst f1⌝ }}}.
+                           ⌜ (k = 1) /\ (Z.of_nat (length s) = (two14 - 1)%Z)%Z \/ (k = 0) /\ (length s < two14 - 1)%Z ⌝ ∗
+          ↪[frame] f0 }}}.
 Proof.
   iIntros "!>" (Φ) "(%Hinst & %Hlocv & Hf & Hstack) HΦ" => /=.
-  
-  rewrite separate4.
-  iApply wp_seq.
-  instantiate (1 := λ x,  (⌜ x = immV [] ⌝ ∗ isStack v s n ∗ ↪[frame] f0)%I).
-  iSplitR; first by iIntros "(%H & _)".
-  iSplitL "Hstack Hf"; first by iApply (is_stack_valid with "[$Hstack $Hf]").
-  iIntros (w) "(-> & Hstack & Hf)".
-  simpl.
-  
-  rewrite separate3.
-  iApply wp_seq.
-  instantiate (1 := λ x,  (⌜ x = immV [] ⌝ ∗ isStack v s n ∗ ↪[frame] f0)%I).
-  iSplitR; first by iIntros "(%H & _)".
-  iSplitL "Hstack Hf"; first by iApply (is_stack_bound_valid with "[$Hstack $Hf]").
-  iIntros (w) "(-> & Hstack & Hf)".
-  simpl.
   
   rewrite separate3.
   iApply wp_seq.
@@ -101,43 +86,10 @@ Proof.
     iSimpl.
     rewrite separate4.
     iApply wp_seq.
- (*   iDestruct "Hstack" as "(%Hdiv & %Hvb & %Hlen & Hv & Hs & Hrest)".
-    iSplitR; last iSplitL "Hf Hv".
-    2: {
-      rewrite separate2.
-      iApply wp_val_app => //.
-      iSplitR.
-      2: {
-        iApply (wp_wand with "[Hf Hv]").
-        iApply wp_load => //.
-        2: {
-          iFrame "Hf".
-          iSplitR; last first.
-          iDestruct (i32_wms with "Hv") as "Hv" => //.
-          rewrite N.add_0_r => /=.
-          rewrite Wasm_int.Int32.Z_mod_modulus_eq.
-          rewrite Z.mod_small; last by unfold ffff0000 in Hvb; rewrite u32_modulus; lias.
-          by instantiate (1 := VAL_int32 _) => /=.
-          by instantiate (1 := λ v, ⌜ v = immV _ ⌝%I).
-        }
-        { done. }
-        iIntros (w) "((-> & Hv) & Hf)" => /=.
-        rewrite N.add_0_r.
-        instantiate (1 := λ v, (⌜ v = immV _ ⌝ ∗ (N.of_nat ↦[wms][Z.to_N _] _) ∗ ↪[frame] _)%I).
-        iFrame "Hf".
-        
-        
-        
-          
-          simpl.
-        iDestruct (wp_load with "[] [$Hf]") as "HWP".
-        iApply wp_load => //.*)
     instantiate ( 1 := λ x, ((((⌜ x = immV [value_of_int 1 ; value_of_int 0 ;
                                             value_of_int (v + length s * 4)%Z] ⌝
                                           ∗ [∗ list] i↦w ∈ s,
-                                N.of_nat n ↦[i32][ Z.to_N (v + length s * 4 - 4 * i)] w) ∗
-
-                                                                                                 (∃ bs, ⌜ (Z.of_nat (length bs) = two16 - 4 - length s * 4)%Z ⌝ ∗ N.of_nat n↦[wms][Z.to_N (v + length s * 4) + 4] bs)
+                                N.of_nat n ↦[i32][ Z.to_N (v + length s * 4 - 4 * i)] w) ∗ (∃ bs, ⌜ (Z.of_nat (length bs) = two16 - 4 - length s * 4)%Z ⌝ ∗ N.of_nat n↦[wms][Z.to_N (v + length s * 4) + 4] bs)
                               )
                                            ∗  N.of_nat n↦[wms][(Wasm_int.N_of_uint i32m (Wasm_int.int_of_Z i32m v) + N.zero)]bits (value_of_int (v + length s * 4)) )
                                ∗ ↪[frame] f0)%I).
@@ -215,10 +167,17 @@ Proof.
       iApply "HΦ".
       iExists _.
       iSplit => //.
-      iFrame "Hstack".
-      iSplit => //; last by iExists f0; iFrame "Hf".
+      iFrame "Hstack Hf".
       iPureIntro.
-      by left.
+      left; split => //.
+      remember (length s) as x.
+      rewrite - Heqx.
+      unfold two14, two16 in *.
+      destruct Hdiv as [m Hdiv].
+      subst v.
+      rewrite Z.add_comm Z_mod_plus_full in Heqmodres.
+      rewrite Z.mod_small in Heqmodres; last by lias.
+      by lias.
     }
     { rewrite Wasm_int.Int32.eq_false => //=; last first.
       { move => H.
@@ -246,10 +205,9 @@ Proof.
       iApply "HΦ".
       iExists _.
       iSplit => //.
-      iFrame "Hstack".
-      iSplit => //; last by iExists f0; iFrame "Hf".
+      iFrame "Hstack Hf".
       iPureIntro.
-      right.
+      right; split => //.
       remember (length s) as x.
       rewrite - Heqx.
       clear - Hlen Heqmodres n0 Hdiv.
@@ -262,6 +220,39 @@ Proof.
     }
 Qed.    
     
+Lemma spec_is_full f0 n (v : Z) (s : seq.seq i32) E: 
+  ⊢ {{{ ⌜ f0.(f_inst).(inst_memory) !! 0 = Some n ⌝ ∗
+        ⌜ (f_locs f0) !! 0 = Some (value_of_int v) ⌝ ∗ 
+        ↪[frame] f0 ∗
+        isStack v s n }}}
+    to_e_list is_full @ E
+    {{{ w, ∃ k, ⌜ w = immV [value_of_int k] ⌝ ∗ isStack v s n ∗
+                           ⌜ (k = 1) /\ (Z.of_nat (length s) = (two14 - 1)%Z)%Z \/ (k = 0) /\ (length s < two14 - 1)%Z ⌝ ∗
+                ↪[frame] f0 }}}.
+Proof.
+  iIntros "!>" (Φ) "(%Hinst & %Hlocv & Hf & Hstack) HΦ" => /=.
+  
+  rewrite separate4.
+  iApply wp_seq.
+  instantiate (1 := λ x,  (⌜ x = immV [] ⌝ ∗ isStack v s n ∗ ↪[frame] f0)%I).
+  iSplitR; first by iIntros "(%H & _)".
+  iSplitL "Hstack Hf"; first by iApply (is_stack_valid with "[$Hstack $Hf]").
+  iIntros (w) "(-> & Hstack & Hf)".
+  simpl.
+  
+  rewrite separate3.
+  iApply wp_seq.
+  instantiate (1 := λ x,  (⌜ x = immV [] ⌝ ∗ isStack v s n ∗ ↪[frame] f0)%I).
+  iSplitR; first by iIntros "(%H & _)".
+  iSplitL "Hstack Hf"; first by iApply (is_stack_bound_valid with "[$Hstack $Hf]").
+  iIntros (w) "(-> & Hstack & Hf)".
+  simpl.
+
+  by iApply (spec_is_full_op with "[$Hf $Hstack] [HΦ]") => //.
+Qed.
+
+
+
 End specs.
 
 
