theories/iris/examples/stack/function/push.v
@@ -4,7 +4,7 @@ From iris.proofmode Require Import base tactics classes.
 From iris.base_logic Require Export gen_heap ghost_map proph_map na_invariants.
 From iris.base_logic.lib Require Export fancy_updates.
 From iris.bi Require Export weakestpre.
-Require Export stack_common.
+Require Export stack_common is_full.
 
 Set Implicit Arguments.
 Unset Strict Implicit.
@@ -19,141 +19,52 @@ Section stack.
   
   Section code.
 
+(*
+  push: [i32, i32] -> []
+  locals declared: [i32]
+
+  Given a stack pointer and an i32, push the i32 to the top of the stack.
+
+  Implementation contains the is_full check which results in a trap if the stack is full. Otherwise, load the 
+  stack top pointer from the stack pointer address, increment it by 4, store the given i32 to the new cell and 
+  update the stack top pointer. Does not cause u32 overflow when the stack pointer is at the last page 
+  of memory.
+  
+  Returns nothing. Can trap only if the stack pointer is invalid or the stack is full.
+
+  Parameters/Locals:
+  0 (input)     stack pointer
+  1 (input)     i32 value to be pushed
+  2             temporary variable storing the new address of the stack top pointer
+*)
     Definition push_op :=
-      [BI_get_local 1 ;
-       BI_load T_i32 None N.zero N.zero ;
-       BI_tee_local 2 ;
-       i32const 65536;
-       BI_binop T_i32 (Binop_i (BOI_rem SX_U)) ;
-       BI_if (Tf [] []) [] [BI_unreachable] ;
-       BI_get_local 2 ;
+      is_full_op ++ 
+     [
+       BI_if (Tf [] []) [BI_unreachable] [];
        BI_get_local 0 ;
-       BI_store T_i32 None N.zero N.zero ;
-       BI_get_local 1 ;
-       BI_get_local 2 ;
+       BI_load T_i32 None N.zero N.zero ;
        i32const 4 ;
        BI_binop T_i32 (Binop_i BOI_add) ;
+       BI_tee_local 2 ;
+       BI_get_local 1 ;
+       BI_store T_i32 None N.zero N.zero ;
+       BI_get_local 0 ;
+       BI_get_local 2 ;
        BI_store T_i32 None N.zero N.zero
       ].
         
     Definition push :=
-      validate_stack 1 ++ push_op.
+      validate_stack 0 ++ validate_stack_bound 0 ++ push_op.
 
   End code.
 
   Section specs.
 
-    Lemma push_not_full v (s: list i32) f E:
-      (two16 | v)%Z ->  
-      (length s < two14 - 1)%Z ->
-      ↪[frame] f ⊢
-        WP [AI_basic (BI_const (value_of_int (v + 4 + length s * 4))); AI_basic (i32const 65536);
-            AI_basic (BI_binop T_i32 (Binop_i (BOI_rem SX_U))); AI_basic (BI_if (Tf [] []) [] [BI_unreachable])] @ E
-        {{ w, ⌜ w = immV [] ⌝ ∗ ↪[frame] f }}.
-    Proof.
-      move => Hdiv Hsize.
-      iIntros "Hf".
-      rewrite separate3.
-      iApply wp_seq.
-      instantiate (1 := λ w, (⌜ w = immV [ _ ]⌝ ∗ ↪[frame] f)%I).
-      iSplitR; first by iIntros "(%H & _)".
-      iSplitL "Hf"; first by iApply (wp_binop with "Hf") => //.
-      iIntros (w) "(-> & Hf)".
-      iApply (wp_if_true with "Hf").
-      {
-        unfold Wasm_int.Int32.modu.
-        simpl.
-        move => Hcontra.
-        apply Znumtheory.Zdivide_mod in Hdiv.
-        assert ((4 + length s * 4 < 65536)%Z) as Hsub.
-        { unfold two14 in Hsize. by lias. }
-        assert ((4 <= 4 + length s * 4)%Z) as Hslb.
-        { by lias. }
-        unfold Wasm_int.Int32.zero in Hcontra.
-        apply Wasm_int.Int32.repr_inv in Hcontra => //=.
-        { 
-          rewrite Wasm_int.Int32.Z_mod_modulus_eq in Hcontra.
-          unfold Wasm_int.Int32.modulus, Wasm_int.Int32.wordsize, Integers.Wordsize_32.wordsize in Hcontra.
-          rewrite <- Znumtheory.Zmod_div_mod in Hcontra => //; last by apply Znumtheory.Zmod_divide => //.
-          unfold two16 in Hdiv.
-          rewrite - Z.add_assoc in Hcontra.
-          rewrite Zplus_mod Hdiv Z.add_0_l in Hcontra.
-          rewrite Z.mod_mod in Hcontra => //.
-          rewrite Z.mod_small in Hcontra; first by lias.
-          split; by lias.
-        }
-        rewrite Wasm_int.Int32.Z_mod_modulus_eq.
-        unfold Wasm_int.Int32.modulus, Wasm_int.Int32.wordsize, Integers.Wordsize_32.wordsize.
-        rewrite <- Znumtheory.Zmod_div_mod => //; last by apply Znumtheory.Zmod_divide => //.
-        rewrite - Z.add_assoc.
-        rewrite Zplus_mod Hdiv Z.add_0_l.
-        rewrite Z.mod_mod => //.
-        remember (4 + length s * 4)%Z as x.
-        rewrite - Heqx.
-        split.
-        { 
-          assert ((0 <= x `mod` 65536)%Z); first by apply Z_mod_pos.
-          by lias.
-        }
-        assert ((x `mod` 65536 < 65536)%Z); first by apply Z_mod_lt.
-        replace (two_power_nat 32) with (4294967296)%Z => //.
-        by lias.
-      }
-      iIntros "!> Hf".
-      replace ([AI_basic (BI_block (Tf [] []) [])]) with ([] ++ [AI_basic (BI_block (Tf [] []) [])]) => //.
-      iApply (wp_block with "Hf") => //.
-      iIntros "!> Hf".
-      by iApply (wp_label_value with "Hf").
-    Qed.
-
-    Lemma push_full v (s: list i32) f E:
-      (0 ≤ v ≤ ffff0000)%Z ->
-      (two16 | v)%Z ->  
-      (Z.of_nat (length s) = two14 - 1)%Z ->
-      ↪[frame] f ⊢
-        WP [AI_basic (BI_const (value_of_int (v + 4 + length s * 4))); AI_basic (i32const 65536);
-            AI_basic (BI_binop T_i32 (Binop_i (BOI_rem SX_U))); AI_basic (BI_if (Tf [] []) [] [BI_unreachable])] @ E
-        {{ w, ⌜ w = trapV ⌝ ∗ ↪[frame] f }}.
-    Proof.
-      move => Hoverflow Hdiv Hsize.
-      iIntros "Hf".
-      rewrite separate3.
-      iApply wp_seq.
-      instantiate (1 := λ w, (⌜ w = immV [ _ ]⌝ ∗ ↪[frame] f)%I).
-      iSplitR; first by iIntros "(%H & _)".
-      iSplitL "Hf"; first by iApply (wp_binop with "Hf") => //.
-      iIntros (w) "(-> & Hf)".
-      iApply (wp_if_false with "Hf").
-      { unfold Wasm_int.Int32.modu. simpl.
-        rewrite Wasm_int.Int32.Z_mod_modulus_eq.
-        fold two16.
-        rewrite Hsize.
-        rewrite - Z.add_assoc.
-        assert (4 + (two14 - 1) * 4 = two16)%Z as ->;[lias|].
-        rewrite - Znumtheory.Zmod_div_mod;try lias.
-        f_equal. apply Znumtheory.Zdivide_mod.
-        apply Z.divide_add_r;auto. apply Z.divide_refl.
-        apply two16_div_i32.
-      }
-      iIntros "!> Hf".
-      take_drop_app_rewrite 0.
-      iApply (wp_block with "Hf") => //.
-      iIntros "!> Hf /=".
-      build_ctx [AI_basic BI_unreachable].
-      iApply wp_label_bind.
-      iApply (wp_wand _ _ _ (λ v, ⌜v = trapV⌝ ∗ _)%I with "[Hf]").
-      iApply (wp_unreachable with "[$]");auto.
-      iIntros (w) "[-> Hf]".
-      deconstruct_ctx.
-      iApply (wp_label_trap with "Hf");auto.
-    Qed.
-    
-    Lemma spec_op_push f0 n v (a : i32) s E :
+    Lemma spec_push_op f0 n v (a : i32) s E :
       ⊢ {{{ ⌜ f0.(f_inst).(inst_memory) !! 0 = Some n ⌝
-          ∗ ⌜ f0.(f_locs) !! 0 = Some (VAL_int32 a) ⌝ 
-          ∗ ⌜ f0.(f_locs) !! 1 = Some (value_of_int v) ⌝
+          ∗ ⌜ f0.(f_locs) !! 0 = Some (value_of_int v) ⌝
+          ∗ ⌜ f0.(f_locs) !! 1 = Some (VAL_int32 a) ⌝ 
           ∗ ⌜ length f0.(f_locs) >= 3 ⌝
-          ∗ ⌜ (0 <= v <= Wasm_int.Int32.max_unsigned - 4 - S (length s) * 4 )%Z ⌝
           ∗ ⌜ (length s < two14 - 1)%Z ⌝
           ∗ isStack v s n
           ∗ ↪[frame] f0 }}}
@@ -162,10 +73,48 @@ Section stack.
                        isStack v (a :: s) n ∗
                        ∃ f1, ↪[frame] f1 ∗ ⌜ f_inst f0 = f_inst f1 ⌝ }}}. 
     Proof.
-      iIntros "!>" (Φ) "(%Hinst & %Hloca & %Hlocv & %Hlocs & %Hv & %Hlens & Hstack & Hf) HΦ" => /=.
-      simpl.
+      iIntros "!>" (Φ) "(%Hinst & %Hlocv & %Hloca & %Hlocs & %Hlens & Hstack & Hf) HΦ" => /=.
+      
+      rewrite (separate9 (AI_basic _)).
+      iApply wp_seq.
+      iSplitR; last iSplitL "Hf Hstack".
+      2: { iApply (spec_is_full_op with "[$Hf $Hstack] []") => //.
+           iIntros (w).
+           instantiate (1 := λ w, (∃ k : Z, ⌜w = immV [value_of_int k]⌝ ∗ isStack v s n ∗ ⌜(k = 1 ∧ (Z.of_nat (length s)) = (two14 - 1)%Z) ∨ k = 0 ∧ (length s < two14 - 1)%Z⌝ ∗ ↪[frame] f0)%I).
+           auto.
+      }
+      { iIntros "H".
+        by iDestruct "H" as (k) "(%Habs & ?)".
+      }           
+
+      iIntros (w) "H".
+      iDestruct "H" as (k) "(-> & Hstack & %Hret & Hf)".
+      destruct Hret as [Hret | Hret] => //.
+      { destruct Hret as [-> Hlens'].
+        rewrite Hlens' in Hlens.
+        by lias.
+      }
+
+      destruct Hret as [-> _] => /=.
+
+      rewrite separate2.
+      iApply wp_seq.
+      instantiate (1 := λ w, (⌜ w = immV [ ]⌝ ∗ ↪[frame] f0)%I).
+      iSplitR; first by iIntros "(%H & _)".
+      iSplitL "Hf".
+      iApply (wp_if_false with "Hf") => //.
+      { iIntros "!> Hf".
+        take_drop_app_rewrite 0.
+        iApply (wp_block with "Hf") => //.
+        iIntros "!> Hf /=".
+        by iApply (wp_label_value with "Hf").
+      }
+
+      iIntros (w) "(-> & Hf)" => /=.
+
       rewrite (separate1 (AI_basic _)).
       iApply wp_seq.
+      
       instantiate (1 := λ x, (⌜ x = immV [value_of_int v] ⌝ ∗ ↪[frame] f0)%I).
       iSplitR ; first by iIntros "[%Habs _]".
       iSplitL "Hf".
@@ -174,16 +123,16 @@ Section stack.
         simpl.
         rewrite separate2.
         iApply wp_seq.
-        instantiate ( 1 := λ x, ((((⌜ x = immV [ value_of_int (v + 4 + length (s) * 4)%Z] ⌝
+        instantiate ( 1 := λ x, ((((⌜ x = immV [ value_of_int (v + (length s) * 4)%Z] ⌝
                                             ∗ [∗ list] i↦w ∈  s,
-                                     N.of_nat n ↦[i32][ Z.to_N (v + 4 + length (s) * 4 - 4 - 4 * i)] w) ∗
+                                     N.of_nat n ↦[i32][ Z.to_N (v + (length s) * 4 - 4 * i)] w) ∗
 
-                                     (∃ bs, ⌜ Z.of_nat (length bs) = (two16 - 4 - length s * 4)%Z ⌝ ∗ N.of_nat n↦[wms][Z.to_N (v + 4 + length s * 4)]bs)
+                                     (∃ bs, ⌜ Z.of_nat (length bs) = (two16 - 4 - length s * 4)%Z ⌝ ∗ N.of_nat n↦[wms][Z.to_N (v + length s * 4) + 4]bs)
                                   )
-                                    ∗  N.of_nat n↦[wms][(Wasm_int.N_of_uint i32m (Wasm_int.int_of_Z i32m v) + N.zero)%N]bits (value_of_int (v + 4 + length (s) * 4)) )
+                                    ∗  N.of_nat n↦[wms][(Wasm_int.N_of_uint i32m (Wasm_int.int_of_Z i32m v) + N.zero)%N]bits (value_of_int (v + length s * 4)) )
                                    ∗ ↪[frame] f0)%I).
         iSplitR ; first by iIntros "[[[[%Habs _] _] _] _]".
-        iDestruct "Hstack" as "(%Hdiv & %Hoverflo & %Hlen & Hv & Hs & Hrest)".
+        iDestruct "Hstack" as "(%Hdiv & %Hvb & %Hlen & Hv & Hs & Hrest)".
         iSplitR "HΦ".
       - iApply wp_load => //.
         iSplitL "Hs Hrest".
@@ -193,8 +142,9 @@ Section stack.
         rewrite N.add_0_r.
         iSimpl.
         rewrite Wasm_int.Int32.Z_mod_modulus_eq.
-        rewrite Z.mod_small ; last by unfold Wasm_int.Int32.max_unsigned in Hv ; lia.
+        rewrite Z.mod_small ; last by unfold ffff0000 in Hvb ; rewrite u32_modulus; lia.
         by iDestruct (i32_wms with "Hv") as "Hv" => //.
+
       - iIntros (w) "[[[[->  Hs] Hrest] Hp] Hf]".
         iSimpl.
         iAssert (isStack v (s) n)%I with "[Hrest Hp Hs]" as "Hstack".
@@ -203,20 +153,45 @@ Section stack.
         rewrite N.add_0_r.
         simpl.
         rewrite Wasm_int.Int32.Z_mod_modulus_eq.
-        rewrite Z.mod_small ; last by unfold Wasm_int.Int32.max_unsigned in Hv ; lia.
+        rewrite Z.mod_small ; last by unfold ffff0000 in Hvb ; rewrite u32_modulus; lia.
         repeat iSplit => //=.
-        iApply i32_wms => //.
-      - rewrite separate2.
+        by iApply i32_wms => //.
+      - rewrite separate3.
         iApply (wp_seq _ _ _ (λ x, (⌜ x = immV [value_of_int (v + 4 + length s * 4)] ⌝
                                             ∗ ↪[frame] _)%I)).
         iSplitR ; first by iIntros "[%Habs _]".
         iSplitL "Hf".
-      - iApply (wp_tee_local with "Hf").
-        iIntros "!> Hf".
-        rewrite separate1.
-        iApply wp_val_app => //.
-        iSplitR ; first by iIntros "!> [%Habs _]".
-        iApply (wp_set_local with "[] [$Hf]") => //=.
+        iApply (wp_binop with "Hf") => //.
+        iIntros "!>".
+        iPureIntro.
+        unfold value_of_int => /=.
+        repeat f_equal.
+        unfold Wasm_int.Int32.iadd, Wasm_int.Int32.add => /=.
+        f_equal.
+        rewrite Wasm_int.Int32.Z_mod_modulus_eq.
+        rewrite Z.mod_small ; first by lias.
+        rewrite u32_modulus.
+        unfold ffff0000 in Hvb.
+        unfold two14 in Hlen.
+        remember (length s) as x.
+        rewrite -Heqx.
+        by lias.
+      - iIntros (w) "[-> Hf]".
+        simpl.
+
+        rewrite separate2.
+        iApply wp_seq; iSplitR; last iSplitL "Hf".
+        instantiate (1 := λ w, (⌜ w = immV [value_of_int (v + 4 + length s * 4)] ⌝ ∗ ↪[frame] _) %I).
+        2: {
+             iApply (wp_tee_local with "Hf").
+             iIntros "!> Hf".
+             rewrite separate1.
+             iApply wp_val_app => //.
+             iSplitR; first by iIntros "!> [%Habs _]".
+             iApply (wp_set_local with "[] [$Hf]") => //=.
+        }
+        { by iIntros "(%Habs & _)". }
+        
       - iIntros (w) "[-> Hf]".
         simpl.
 
@@ -224,25 +199,6 @@ Section stack.
                                 (f_locs f0) 2 (value_of_int (v + 4 + length s * 4)) ;
                    f_inst := f_inst f0 |} as f1.
         rewrite - Heqf1.
-        rewrite separate4.
-        iApply wp_seq.
-        instantiate (1 := λ x, (⌜ x = immV []⌝ ∗ ↪[frame] f1 )%I ).
-        iSplitR; first by iIntros "(%H & _)".
-        iSplitL "Hf"; first by iApply (push_not_full with "Hf") => //.
-
-        iIntros (w) "(-> & Hf)".
-        iSimpl.
-
-        rewrite (separate1 (AI_basic (BI_get_local 2))).
-        iApply wp_seq.
-        instantiate (1 := λ x, (⌜ x = immV [value_of_int (v + 4 + length s * 4)] ⌝ ∗ ↪[frame] f1)%I).
-        iSplitR; first by iIntros "(%H & _)".
-        iSplitL "Hf"; first iApply (wp_get_local with "[] [$Hf]") => //.
-        { rewrite Heqf1 => /=.
-          by rewrite set_nth_read. }
-
-        iIntros (w) "(-> & Hf)".
-        simpl.
         rewrite separate2.
         iApply wp_seq.
         instantiate (1 := λ x, (⌜ x = immV [value_of_int (v + 4 + length s * 4) ;
@@ -253,14 +209,15 @@ Section stack.
         iApply wp_val_app => //.
         iSplitR ; first by iIntros "!> [%Habs _]".
         subst f1 ; iApply (wp_get_local with "[] [$Hf]") => //.
-        unfold set_nth.
-        destruct (f_locs f0) => //=.
+        simpl.
+        rewrite - fmap_insert_set_nth; last by lias.
+        by rewrite list_lookup_insert_ne => //.
       - iIntros (w) "[-> Hf]".
         iSimpl.
         rewrite separate3.
         iApply wp_seq.
         instantiate
-          (1 := λ x, (((⌜ x = immV [] ⌝ ∗ N.of_nat n↦[i32][ Z.to_N v] Wasm_int.Int32.repr (v+4+length s * 4) ∗ ([∗ list] i↦w ∈ s, N.of_nat n↦[i32][Z.to_N (v + 4 + length s * 4 - 4 - 4 * i)] w) ∗ (∃ bs, ⌜ Z.of_nat (length bs) = (two16 - 4 - length (s) * 4 - 4)%Z ⌝ ∗ N.of_nat n↦[wms][Z.to_N (v + 4 + S (length s) * 4)]bs) )
+          (1 := λ x, (((⌜ x = immV [] ⌝ ∗ N.of_nat n↦[i32][ Z.to_N v] Wasm_int.Int32.repr (v+length s * 4) ∗ ([∗ list] i↦w ∈ s, N.of_nat n↦[i32][Z.to_N (v + length s * 4 - 4 * i)] w) ∗ (∃ bs, ⌜ Z.of_nat (length bs) = (two16 - 4 - length (s) * 4 - 4)%Z ⌝ ∗ N.of_nat n↦[wms][Z.to_N (v + 4 + S (length s) * 4)]bs) )
                          ∗ N.of_nat n ↦[wms][Wasm_int.N_of_uint i32m (Wasm_int.int_of_Z i32m (v + 4 + length s * 4)%Z) + N.zero]bits (VAL_int32 a)) ∗ ↪[frame] f1)%I).
         iSplitR ; first by iIntros "[[[ %Habs _ ] _] _]". 
         iDestruct "Hstack" as "(_ & _ & _ & Hp & Hs & Hrest)".
@@ -268,6 +225,7 @@ Section stack.
         unfold two16 in Hbs.
         unfold two14 in Hlens.
         remember (length s) as x.
+        rewrite - Heqx.
         do 4 (destruct bs ; first by exfalso ; clear Heqx s ; simpl in Hbs ; lia).
         rewrite separate4.
         unfold mem_block_at_pos at 1.
@@ -280,11 +238,7 @@ Section stack.
         iNext.
         simpl.
         subst x.
-        by instantiate (1 := λ x, (⌜ x = immV [] ⌝ ∗ N.of_nat n ↦[i32][ Z.to_N v] Wasm_int.Int32.repr (v + 4 + length s * 4) ∗ ([∗ list] i↦w ∈ s, N.of_nat n
-                                                                                                                                                    ↦[i32][ Z.to_N (v + 4 + length s * 4 - 4 - 4 * i)] w) ∗ ([∗ list] k↦y ∈ bs, N.of_nat n↦[wm][N.of_nat
-                                                                                                                                                                                                                                                  (N.to_nat
-                                                                                                                                                                                                                                                     (Z.to_N (v + 4 + length s * 4)) +
-                                                                                                                                                                                                                                                     S (S (S (S k))))]y))%I);
+        by instantiate (1 := λ x, (⌜ x = immV [] ⌝ ∗ N.of_nat n ↦[i32][ Z.to_N v] Wasm_int.Int32.repr (v + length s * 4) ∗ ([∗ list] i↦w ∈ s, N.of_nat n ↦[i32][ Z.to_N (v + length s * 4 - 4 * i)] w) ∗ ([∗ list] k↦y ∈ bs, N.of_nat n↦[wm][N.of_nat (N.to_nat (Z.to_N (v + length s * 4)+4) + S (S (S (S k))))]y))%I);
         iFrame.
         3: instantiate (1 := [b ; b0 ; b1 ; b2]) => //=. 
         3: done.
@@ -296,13 +250,13 @@ Section stack.
         rewrite Wasm_int.Int32.Z_mod_modulus_eq Z.mod_small.
         rewrite of_nat_to_nat_plus.
         rewrite N.add_0_r.
-        by subst x.
-        unfold Wasm_int.Int32.max_unsigned in Hv.
-        rewrite - Heqx.
+        replace (Z.to_N (v+x*4)+4)%N with (Z.to_N (v+4+x*4)) => //; last by lias.
+        unfold ffff0000 in Hvb.
+        rewrite u32_modulus.
         lia.
-        iIntros (w) "[[(-> & Hp & Hs & Hrest) Ha] Hf]".
+        
+      - iIntros (w) "[[(-> & Hp & Hs & Hrest) Ha] Hf]".
         iFrame.
-        iSplitR "Ha".
         iSplit ; first done.
         subst x ; iFrame.
         iExists bs.
@@ -316,13 +270,10 @@ Section stack.
         do 2 rewrite of_nat_to_nat_plus.
         remember (length s) as y.
         clear Heqy s.
-        replace (Z.to_N (v + 4 + y * 4) + N.of_nat (S (S (S (S k)))))%N with
-          (Z.to_N (v + 4 + S y * 4) + N.of_nat k)%N.
-        done.
+        replace (Z.to_N (v + y * 4) + 4 + N.of_nat (S (S (S (S k)))))%N with
+          (Z.to_N (v + 4 + S y * 4) + N.of_nat k)%N => //.
         lia.
-        by subst x.
       - iIntros (w) "[[(-> & Hp & Hs & Hrest) Ha] Hf]".
-        unfold of_val, fmap, list_fmap.
         iSimpl.
         rewrite (separate1 (AI_basic _)).
         iApply wp_seq.
@@ -331,11 +282,10 @@ Section stack.
         iSplitL "Hf".
       - iApply (wp_get_local with "[] [$Hf]") => //.
         subst f1 => //=.
-        unfold set_nth.
-        destruct (f_locs f0) => //=.
-        destruct l => //=.
+        rewrite - fmap_insert_set_nth; last by lias.
+        by rewrite list_lookup_insert_ne => //.
+          
       - iIntros (w) "[-> Hf]".
-        unfold of_val, fmap, list_fmap.
         iSimpl.
         rewrite separate2.
         iApply wp_seq.
@@ -351,48 +301,21 @@ Section stack.
         subst f1 => //=.
         rewrite set_nth_read => //=.
         by subst x.
+          
       - iIntros (w) "[-> Hf]".
-        unfold of_val, fmap, list_fmap.
-        iSimpl.
-        rewrite separate4.
-        iApply wp_seq.
-        instantiate (1 := λ x, ( ⌜ x = immV [value_of_int v ;
-                                             value_of_int ( v + 4 + S (length s) * 4 )] ⌝
-                                         ∗ ↪[frame] f1)%I).
-        iSplitR ; first by iIntros "[%Habs _]".
-        iSplitL "Hf".
-      - rewrite separate1.
-        iApply wp_val_app => //.
-        iSplitR ; first by iIntros "!> [%Habs _]".
-        iApply (wp_binop with "Hf") => //=.
-        iPureIntro.
-        unfold Wasm_int.Int32.iadd, Wasm_int.Int32.add.
-        rewrite Wasm_int.Int32.unsigned_repr.
-        rewrite Wasm_int.Int32.unsigned_repr.
-        unfold value_of_int => //=.
-        rewrite - Heqx.
-        replace (v + 4 + x * 4 + 4)%Z with (v + 4 + S x * 4)%Z => //=.
-        lia.
-        unfold Wasm_int.Int32.max_unsigned, Wasm_int.Int32.modulus.
-        unfold Wasm_int.Int32.wordsize, Integers.Wordsize_32.wordsize.
-        replace (two_power_nat 32) with two32 ; last done.
-        unfold two32 ; lia.
-        rewrite - Heqx. lia.
-      - iIntros (w) "[-> Hf]".
-        unfold of_val, fmap, list_fmap.
         iSimpl.
         iApply wp_wand_r.
         iSplitL "Hf Hp".
       - iApply wp_store.
         done.
-        instantiate (1 := bits (value_of_int (v + 4 + length s * 4))) => //=.
+        instantiate (1 := bits (value_of_int (v + length s * 4))) => //=.
         instantiate (2 := f1).
         subst f1 => //=.
         instantiate (1 := λ x, ⌜ x = immV [] ⌝%I).
         iFrame.
         iSplit => //=.
         rewrite Wasm_int.Int32.Z_mod_modulus_eq.
-        rewrite Z.mod_small ; last by unfold Wasm_int.Int32.max_unsigned in Hv ; lia.
+        rewrite Z.mod_small ; last by unfold ffff0000 in Hvb ; rewrite u32_modulus; lia.
         iDestruct (i32_wms with "Hp") as "Hp" => //.
         rewrite N.add_0_r.
         by subst x.
@@ -405,25 +328,28 @@ Section stack.
         iPureIntro ; rewrite - Heqx ; clear Heqx s ; unfold two14 ; lia.
         iSplitL "Hp".
         rewrite Wasm_int.Int32.Z_mod_modulus_eq.
-        rewrite Z.mod_small ; last by unfold Wasm_int.Int32.max_unsigned in Hv ; lia.
+        rewrite Z.mod_small ; last by unfold ffff0000 in Hvb ; rewrite u32_modulus; lia.
         iApply i32_wms => //.
         rewrite N.add_0_r.
-        unfold value_of_int => //=.
+        rewrite -Heqx.
+        replace (v+4+x*4)%Z with (v+S x * 4)%Z => //.
+        by lias.
+        
         iSplitR "Hrest".
         iSplitL "Ha".
         iApply i32_wms => //.
         rewrite Wasm_int.Int32.Z_mod_modulus_eq.
-        rewrite Z.mod_small ; last by unfold Wasm_int.Int32.max_unsigned in Hv ; lia.
+        rewrite Z.mod_small ; last by unfold ffff0000 in Hvb ; rewrite u32_modulus; lia.
         rewrite N.add_0_r.
         rewrite - Heqx.
-        replace (v + 4 + S x * 4 - 4 - 4 * 0%nat)%Z
+        replace (v + S x * 4 - 4 * 0%nat)%Z
           with (v + 4 + x * 4)%Z ; last lia.
         done.
         iApply (big_sepL_impl with "Hs").
         iIntros "!>" (k y) "%Hbits H".
         rewrite - Heqx.
-        replace (v + 4 + S x * 4 - 4 - 4 * S k)%Z
-          with  (v + 4 + x * 4 - 4 - 4 * k)%Z ; last lia.
+        replace (v + S x * 4 - 4 * S k)%Z
+          with  (v + x * 4 - 4 * k)%Z ; last lia.
         done.
         iDestruct "Hrest" as (bs0) "[%Hbs0 Hrest]".
         iExists bs0.
@@ -431,16 +357,19 @@ Section stack.
         iPureIntro.
         rewrite - Heqx.
         lia.
-        by subst x.
+        rewrite - Heqx.
+        replace (Z.to_N (v+4+S x*4)) with (Z.to_N (v+S x * 4) + 4)%N => //.
+        by lias.
+        subst x.
         iExists _ ; by subst ; iFrame.
     Qed.
 
+    
     Lemma spec_push f0 n v (a : i32) s E :
       ⊢ {{{ ⌜ f0.(f_inst).(inst_memory) !! 0 = Some n ⌝
-          ∗ ⌜ f0.(f_locs) !! 0 = Some (VAL_int32 a) ⌝ 
-          ∗ ⌜ f0.(f_locs) !! 1 = Some (value_of_int v) ⌝
+          ∗ ⌜ f0.(f_locs) !! 0 = Some (value_of_int v) ⌝
+          ∗ ⌜ f0.(f_locs) !! 1 = Some (VAL_int32 a) ⌝ 
           ∗ ⌜ length f0.(f_locs) >= 3 ⌝
-          ∗ ⌜ (0 <= v <= Wasm_int.Int32.max_unsigned - 4 - S (length s) * 4 )%Z ⌝
           ∗ ⌜ (length s < two14 - 1)%Z ⌝
           ∗ isStack v s n
           ∗ ↪[frame] f0 }}}
@@ -449,14 +378,23 @@ Section stack.
                        isStack v (a :: s) n ∗
                        ∃ f1, ↪[frame] f1 ∗ ⌜ f_inst f0 = f_inst f1 ⌝ }}}. 
     Proof.
-      iIntros "!>" (Φ) "(%Hinst & %Hloca & %Hlocv & %Hlocs & %Hv & %Hlens & Hstack & Hf) HΦ" => /=.
+      iIntros "!>" (Φ) "(%Hinst & %Hlocv & %Hloca & %Hlocs & %Hlens & Hstack & Hf) HΦ" => /=.
+      
       rewrite separate4.
       iApply wp_seq.
       instantiate (1 := λ x,  (⌜ x = immV [] ⌝ ∗ isStack v s n ∗ ↪[frame] f0)%I).
       iSplitR; first by iIntros "(%H & _)".
       iSplitL "Hstack Hf"; first by iApply (is_stack_valid with "[$Hstack $Hf]").
+      
       iIntros (w) "(-> & Hstack & Hf) /=".
-      iApply (spec_op_push with "[$Hf $Hstack] [$]").
+      rewrite separate3.
+      iApply wp_seq.
+      instantiate (1 := λ x,  (⌜ x = immV [] ⌝ ∗ isStack v s n ∗ ↪[frame] f0)%I).
+      iSplitR; first by iIntros "(%H & _)".
+      iSplitL "Hstack Hf"; first by iApply (is_stack_bound_valid with "[$Hstack $Hf]").
+      
+      iIntros (w) "(-> & Hstack & Hf) /=".
+      iApply (spec_push_op with "[$Hf $Hstack] [$]").
       auto.
     Qed.
       
